initial commit

AdventOfCode2024/Basic.lean
@@ -1,1 +1,329 @@
-def hello := "world"
+import Std.Data.HashMap.Basic
+import Std.Data.HashSet.Basic
+import Batteries.Data.BinaryHeap
+import Batteries.Data.String.Lemmas
+import Mathlib.Control.Traversable.Basic
+import Mathlib.Control.Fold
+
+@[inline]
+def Function.repeat (f: α → α) (init: α) (n: ℕ) :=
+  match n with
+  | 0 => init
+  | k + 1 => Function.repeat f (f init) k
+
+lemma Option.length_toList: (Option.toList o).length ≤ 1 := by
+  unfold toList
+  split
+  · simp only [List.length_nil, Nat.zero_le]
+  · simp only [List.length_singleton, Nat.le_refl]
+
+instance : DecidableRel Int.lt :=
+  fun x y => by unfold Int.lt; infer_instance
+
+@[inline]
+def Fin.pred' (a: Fin n) :=
+  Fin.mk (↑a - 1) (trans (Nat.pred_le _) a.isLt)
+
+@[inline]
+def Fin.succ' (a: Fin n) (h: a.succ ≠ last n): Fin n :=
+  Fin.castLT (Fin.succ a) (val_lt_last h)
+
+@[inline]
+def Fin.subNat' (a: Fin n) (b: Nat): Fin n :=
+  if h: b ≤ a then a - ⟨b, trans h a.2⟩
+  else ⟨0, Fin.pos a⟩
+
+@[inline]
+def Fin.addNat' (a: Fin n) (b: Nat): Fin n :=
+  if h: a + b < n then ⟨a + b, h⟩
+  else ⟨n - 1, Nat.sub_one_lt_of_lt (Fin.pos a)⟩
+
+/-- Inclusive -/
+@[inline]
+def MLList.finRange [Monad m] (start stop: Fin n): MLList m (Fin n) :=
+  MLList.fix? (fun k => pure (
+    let k' := k.val.succ
+    if h: k' ≤ stop then
+      some ⟨k', trans h stop.isLt⟩
+    else none
+  )) start
+
+@[inline]
+def MLList.length [Monad m] (l: MLList m α) :=
+  MLList.fold (fun n _ => n + 1) 0 l
+
+abbrev Coord (h w: Nat) := Fin h × Fin w
+namespace Coord
+def upperLeft (hpos: 0 < h) (wpos: 0 < w): Coord h w := (⟨0, hpos⟩, ⟨0, wpos⟩)
+def lowerRight (hpos: 0 < h) (wpos: 0 < w): Coord h w :=
+  (⟨h - 1, Nat.sub_one_lt_of_lt hpos⟩, ⟨w - 1, Nat.sub_one_lt_of_lt wpos⟩)
+
+def mk (x y: ℕ) (hx: x < h := by decide) (hy: y < w := by decide): Coord h w :=
+  (⟨x, hx⟩, ⟨y, hy⟩)
+
+def all (h w: Nat): MLList Id (Coord h w) :=
+  (MLList.fin h).bind (fun a =>
+    (MLList.fin w).map (Prod.mk a))
+
+@[inline]
+def neighbors: Coord h w → List (Coord h w)
+| (a, b) =>
+  let l1 := if ↑a = 0 then [] else (a.pred', b) :: []
+  let l2 := if ↑b = 0 then l1 else (a, b.pred') :: l1
+  let l3 := if ha: a.succ = Fin.last h then l2 else (a.succ' ha, b) :: l2
+  let l4 := if hb: b.succ = Fin.last w then l3 else (a, b.succ' hb) :: l3
+  l4
+
+theorem length_neighbors {c: Coord h w}: (neighbors c).length ≤ 4 := by
+  dsimp only [neighbors]
+  split_ifs <;> simp
+
+inductive Facing | north | south | east | west
+deriving BEq, Repr, Hashable, DecidableEq
+
+@[inline]
+def Facing.all :=
+  [north, south, east, west]
+
+def neighborFacing: Coord h w → Facing → Option (Coord h w)
+| (y, x) => fun
+  | .north => if ↑y = 0 then none else some (y.pred', x)
+  | .west  => if ↑x = 0 then none else some (y, x.pred')
+  | .south => if hy: y.succ = Fin.last h then none else (y.succ' hy, x)
+  | .east  => if hx: x.succ = Fin.last w then none else (y, x.succ' hx)
+
+@[inline]
+def taxicabDist: Coord h w → Coord h w → Nat
+| (x₁, y₁), (x₂, y₂) =>
+  (Int.sub x₁ x₂).natAbs + (Int.sub y₁ y₂).natAbs
+
+@[inline]
+def withinTaxicabDist (maxDist: Nat) (c: Coord h w): MLList Id (Coord h w) :=
+  let (cx, cy) := c
+  .finRange
+    (cx.subNat' maxDist)
+    (cx.addNat' maxDist) >>= fun x =>
+    let xDist := (Int.sub cx x).natAbs
+    let maxYDist := maxDist - xDist
+    MLList.finRange
+      (cy.subNat' maxYDist)
+      (cy.addNat' maxYDist)
+    |>.map (x, ·)
+
+end Coord
+
+def Char.toNat?: Char → Option (Fin 10)
+| '0' => some 0 | '1' => some 1 | '2' => some 2
+| '3' => some 3 | '4' => some 4 | '5' => some 5
+| '6' => some 6 | '7' => some 7 | '8' => some 8
+| '9' => some 9 | _ => none
+
+def String.toNat?' (s: String): Except String Nat :=
+  match s.toNat? with
+  | .some n => .ok n
+  | .none => .error s!"could not parse `{s}` to `Nat`"
+
+def String.toInt?' (s: String): Except String ℤ :=
+  match s.toInt? with
+  | some n => .ok n
+  | none => .error s!"Could not parse `{s}` as `Int`"
+
+set_option synthInstance.checkSynthOrder false in
+instance [Repr ε]: MonadLiftT (Except ε) IO where
+  monadLift
+  | .ok x => pure x
+  | .error e => .error (.userError (reprStr e))
+
+instance : MonadLiftT Option IO where
+  monadLift
+  | some x => pure x
+  | none => .error (.userError "Failed to get value in `Option` computation")
+
+def Option.toExcept (msg: String): Option α → Except String α
+| some a => .ok a
+| none => .error msg
+
+def loadAsString (path: System.FilePath) :=
+  IO.FS.withFile path .read
+  (fun handle => do return ← handle.readToEnd)
+
+/-- Split by single newlines.-/
+def load (path: System.FilePath) := do
+  let str ← loadAsString path
+  return str.crlfToLf.splitOn "\n"
+
+/-- Split by double newlines.-/
+def load' (path: System.FilePath) := do
+  let str ← loadAsString path
+  return str.crlfToLf.splitOn "\n\n"
+
+instance [Inhabited α]: Inhabited (Thunk α) :=
+  ⟨.mk (fun () => default)⟩
+
+instance : Monad Thunk where
+  pure := Thunk.pure
+  bind := Thunk.bind
+
+instance : LawfulMonad Thunk := by
+  apply LawfulMonad.mk'
+  all_goals
+    repeat intro
+    rfl
+
+def List.enumFin (l: List α): List (Fin l.length × α) :=
+  l.enum.attach.map (fun ⟨(i, x), h⟩ =>
+    have ⟨hi, _⟩ := List.mem_enum h
+    (⟨i, hi⟩, x))
+
+def Traversable.minBy [Traversable t] (f: α → Option Nat) (l: t α): Option (α × Nat) :=
+  Traversable.foldl
+    (fun acc a =>
+      match (acc, f a) with
+      | (_, .none) => acc
+      | (.none, .some n) => .some (a, n)
+      | (.some (_, m), .some n) =>
+        if m ≤ n then acc else .some (a, n))
+    .none
+    l
+
+def dijkstra [BEq α] [Hashable α] (edges: α → Array (α × Nat)) (src: α) := Id.run do
+  let mut dist: Std.HashMap α Nat := { (src, 0) }
+  let mut prev: Std.HashMap α α := {  }
+  let mut queue: Batteries.BinaryHeap (α × Nat) (·.2 > ·.2) := .insert ∅ (src, 0)
+
+  while true do
+    let max := queue.max
+    queue := queue.popMax
+    match max with
+    | none => break
+    | some (u, uDist) =>
+      for (v, uvEdgeDist) in edges u do
+        let distThrough_uv := uDist + uvEdgeDist
+        let replace := Option.all (distThrough_uv < ·) (dist.get? v)
+        if replace then
+          dist := dist.insert v distThrough_uv;
+          prev := prev.insert v u;
+          queue := queue.insert (v, distThrough_uv)
+    ()
+
+  (dist.get?, prev.get?)
+
+partial def pathTo (dst: α) (prev: α → Option α) :=
+  go dst prev [dst]
+where go dst prev acc :=
+  match prev dst with
+  | none => acc
+  | some next => go next prev (next :: acc)
+
+def Substring.Valid.bsize_drop_one {s: Substring} (h₁: s.Valid) (h₂: ¬s.isEmpty): (s.drop 1).bsize < s.bsize := by
+  rw [Valid.bsize h₁, Valid.bsize (Valid.drop h₁ 1), Valid.data_drop h₁ 1]
+  rw [Valid.isEmpty h₁] at h₂
+  match h: s.toString.data with
+  | [] =>
+    apply False.elim ∘ h₂
+    rw [show s.toString = .mk s.toString.data from rfl, h]
+  | x :: xs =>
+    rw [List.drop_one, List.tail_cons, String.utf8Len_cons, Nat.lt_add_right_iff_pos]
+    exact Char.utf8Size_pos x
+
+def Substring.mapM [Monad m] (f: Char → m α) (s: Substring) (h: s.Valid): m (List α) :=
+  loop s [] h
+where
+  loop s acc (h: s.Valid) :=
+    if s.isEmpty then pure acc.reverse
+    else do
+      loop (s.drop 1) ((←f s.front) :: acc) (Valid.drop h 1)
+  termination_by s.bsize
+  decreasing_by exact Valid.bsize_drop_one h ‹¬s.isEmpty›
+
+def Std.HashSet.inter [BEq α] [Hashable α] (s₁ s₂: Std.HashSet α) :=
+  s₂.filter (· ∈ s₁)
+
+instance [BEq α] [Hashable α]: Inter (Std.HashSet α) where
+  inter := Std.HashSet.inter
+
+inductive Validate (ε: Type u) (α: Type v)
+| ok: α → Validate ε α
+| errors: List ε → Validate ε α
+
+namespace Validate
+instance : Applicative (Validate ε) where
+  pure := .ok
+  seq vf vx :=
+    match vf, vx () with
+    | .ok f, .ok x => .ok (f x)
+    | .ok _, .errors errs => .errors errs
+    | .errors errs, .ok _ => .errors errs
+    | .errors errs₁, .errors errs₂ => .errors (errs₁ ++ errs₂)
+end Validate
+
+namespace Grid
+
+inductive ParseError
+| unknownChar (location: Coord h w) (c: Char)
+deriving Repr
+
+def parse (lines: List String)
+  (hh: lines.length = h) (hw: ∀ line ∈ lines, line.length = w)
+  (f: Coord h w → Char → Option α): Except ParseError (List α) :=
+
+  List.flatten <$>
+  lines.enum.attach.mapM fun ⟨(i, line), hi⟩ =>
+    have ⟨hi, hline⟩ := hh ▸ List.mem_enum hi
+    line.toList.enum.attach.mapM fun ⟨(j, c), hj⟩ =>
+
+      have ⟨hj, _⟩: j < w ∧ _ :=
+        hw line (List.mem_iff_getElem.mpr ⟨i, hh ▸ hi, hline.symm⟩)
+        ▸ (show line.toList.length = line.length from rfl)
+        ▸ List.mem_enum hj
+
+      let coord := (⟨i, hi⟩, ⟨j, hj⟩)
+      match f coord c with
+      | none => .error (.unknownChar coord c)
+      | some a => .ok a
+
+end Grid
+
+structure Maze where
+  h: Nat
+  w: Nat
+  start: Coord h w
+  «end»: Coord h w
+  track: Std.HashSet (Coord h w)
+
+namespace Maze
+
+inductive ParseError
+| base (err: Grid.ParseError)
+| differentLengthRows
+| notOneStart
+| notOneEnd
+deriving Repr
+
+private inductive TileType | start | «end» | track | wall
+deriving DecidableEq
+
+def parse (lines: List String): Except ParseError Maze := do
+  let w := (String.length <$> lines.head?).getD 0
+  if hw: ∀ line ∈ lines, line.length = w then
+    let grid ← Except.mapError .base <|
+      Grid.parse lines rfl hw fun c => fun
+        | 'S' => some (c, TileType.start)
+        | 'E' => some (c, .end)
+        | '.' => some (c, .track)
+        | '#' => some (c, .wall)
+        | _ => none
+    let [(start, _)] := grid.filter fun (_, tt) => tt = .start
+      | .error .notOneStart
+    let [(«end», _)] := grid.filter fun (_, tt) => tt = .end
+      | .error .notOneEnd
+    let track := grid
+      |>.filter (fun (_, tt) =>
+        tt = .start || tt = .end || tt = .track)
+      |>.map Prod.fst
+      |> Std.HashSet.ofList
+
+    return { h := lines.length, w, start, «end», track }
+  else
+    .error .differentLengthRows
+end Maze
