lakefile.lean
@@ -1,6 +1,9 @@
 import Lake
 open Lake DSL
 
+require "leanprover-community" / "batteries" @ git "main"
+require "leanprover-community" / "mathlib" @ git "master"
+
 package «advent-of-code-2024» where
   -- add package configuration options here
 
